<?xml version="1.0"?>
<rdf:RDF xmlns="http://purl.org/ppeo/MDO.owl#"
     xml:base="http://purl.org/ppeo/MDO.owl"
     xmlns:owl="http://www.w3.org/2002/07/owl#"
     xmlns:rdf="http://www.w3.org/1999/02/22-rdf-syntax-ns#"
     xmlns:xml="http://www.w3.org/XML/1998/namespace"
     xmlns:xsd="http://www.w3.org/2001/XMLSchema#"
     xmlns:rdfs="http://www.w3.org/2000/01/rdf-schema#">
    <owl:Ontology rdf:about="http://purl.org/ppeo/MDO.owl"/>
    


    <!-- 
    ///////////////////////////////////////////////////////////////////////////////////////
    //
    // Object Properties
    //
    ///////////////////////////////////////////////////////////////////////////////////////
     -->

    


    <!-- http://purl.org/ppeo/MDO.owl#contains -->

    <owl:ObjectProperty rdf:about="http://purl.org/ppeo/MDO.owl#contains">
        <rdfs:domain rdf:resource="http://purl.org/ppeo/MDO.owl#object"/>
        <rdfs:range rdf:resource="http://purl.org/ppeo/MDO.owl#metadata_entity"/>
        <rdfs:comment xml:lang="en">Expresses a whole-part relation between an object and another object or field which should be reflected in the structure of the interface (e.g. contained fields should be displayed within the containing sections, and contained subsections should be englobed by or linked to their containing sections).</rdfs:comment>
        <rdfs:label xml:lang="en">contains</rdfs:label>
    </owl:ObjectProperty>
    


    <!-- http://purl.org/ppeo/MDO.owl#containsAtLeastOne -->

    <owl:ObjectProperty rdf:about="http://purl.org/ppeo/MDO.owl#containsAtLeastOne">
        <rdfs:subPropertyOf rdf:resource="http://purl.org/ppeo/MDO.owl#contains"/>
        <rdfs:domain rdf:resource="http://purl.org/ppeo/MDO.owl#object"/>
        <rdfs:range rdf:resource="http://purl.org/ppeo/MDO.owl#metadata_entity"/>
        <rdfs:comment xml:lang="en">Indicates that the parent object must contain at least one child entity.</rdfs:comment>
        <rdfs:label xml:lang="en">contains at least one</rdfs:label>
    </owl:ObjectProperty>
    


    <!-- http://purl.org/ppeo/MDO.owl#containsAtMostOne -->

    <owl:ObjectProperty rdf:about="http://purl.org/ppeo/MDO.owl#containsAtMostOne">
        <rdfs:subPropertyOf rdf:resource="http://purl.org/ppeo/MDO.owl#contains"/>
        <rdfs:domain rdf:resource="http://purl.org/ppeo/MDO.owl#object"/>
        <rdfs:range rdf:resource="http://purl.org/ppeo/MDO.owl#metadata_entity"/>
        <rdfs:comment xml:lang="en">Indicates that the parent object can contain at most one child entity.</rdfs:comment>
        <rdfs:label xml:lang="en">contains at most one</rdfs:label>
    </owl:ObjectProperty>
    


    <!-- http://purl.org/ppeo/MDO.owl#containsExactlyOne -->

    <owl:ObjectProperty rdf:about="http://purl.org/ppeo/MDO.owl#containsExactlyOne">
        <rdfs:subPropertyOf rdf:resource="http://purl.org/ppeo/MDO.owl#contains"/>
        <rdfs:domain rdf:resource="http://purl.org/ppeo/MDO.owl#object"/>
        <rdfs:range rdf:resource="http://purl.org/ppeo/MDO.owl#metadata_entity"/>
        <rdfs:comment xml:lang="en">Indicates that the parent object must contain exactly one child entity.</rdfs:comment>
        <rdfs:label xml:lang="en">contains exactly one</rdfs:label>
    </owl:ObjectProperty>
    


    <!-- http://purl.org/ppeo/MDO.owl#containsMoreThanOne -->

    <owl:ObjectProperty rdf:about="http://purl.org/ppeo/MDO.owl#containsMoreThanOne">
        <rdfs:subPropertyOf rdf:resource="http://purl.org/ppeo/MDO.owl#contains"/>
        <rdfs:domain rdf:resource="http://purl.org/ppeo/MDO.owl#object"/>
        <rdfs:range rdf:resource="http://purl.org/ppeo/MDO.owl#metadata_entity"/>
        <rdfs:comment xml:lang="en">Indicates that the parent object must contain more than one child entity.</rdfs:comment>
        <rdfs:label xml:lang="en">contains more than one</rdfs:label>
    </owl:ObjectProperty>
    


    <!-- http://purl.org/ppeo/MDO.owl#includes -->

    <owl:ObjectProperty rdf:about="http://purl.org/ppeo/MDO.owl#includes">
        <rdfs:domain rdf:resource="http://purl.org/ppeo/MDO.owl#object"/>
        <rdfs:range rdf:resource="http://purl.org/ppeo/MDO.owl#metadata_entity"/>
        <rdfs:comment xml:lang="en">Expresses a whole-part relation between an object and an entity that has been previously instanced, to allow the allocation of that instance to the parent object. This should be reflected in the interface displaying a selector of instances of the child object that have been previously entered elsewhere in this metadata form.</rdfs:comment>
        <rdfs:label xml:lang="en">includes</rdfs:label>
    </owl:ObjectProperty>
    


    <!-- http://purl.org/ppeo/MDO.owl#includesAtLeastOne -->

    <owl:ObjectProperty rdf:about="http://purl.org/ppeo/MDO.owl#includesAtLeastOne">
        <rdfs:subPropertyOf rdf:resource="http://purl.org/ppeo/MDO.owl#includes"/>
        <rdfs:domain rdf:resource="http://purl.org/ppeo/MDO.owl#object"/>
        <rdfs:range rdf:resource="http://purl.org/ppeo/MDO.owl#metadata_entity"/>
        <rdfs:comment xml:lang="en">Indicates that the parent object must include at least one child entity.</rdfs:comment>
        <rdfs:label xml:lang="en">includes at least one</rdfs:label>
    </owl:ObjectProperty>
    


    <!-- http://purl.org/ppeo/MDO.owl#includesAtMostOne -->

    <owl:ObjectProperty rdf:about="http://purl.org/ppeo/MDO.owl#includesAtMostOne">
        <rdfs:subPropertyOf rdf:resource="http://purl.org/ppeo/MDO.owl#includes"/>
        <rdfs:domain rdf:resource="http://purl.org/ppeo/MDO.owl#object"/>
        <rdfs:range rdf:resource="http://purl.org/ppeo/MDO.owl#metadata_entity"/>
        <rdfs:comment xml:lang="en">Indicates that the parent object can include at most one child entity.</rdfs:comment>
        <rdfs:label xml:lang="en">includes at most one</rdfs:label>
    </owl:ObjectProperty>
    


    <!-- http://purl.org/ppeo/MDO.owl#includesExactlyOne -->

    <owl:ObjectProperty rdf:about="http://purl.org/ppeo/MDO.owl#includesExactlyOne">
        <rdfs:subPropertyOf rdf:resource="http://purl.org/ppeo/MDO.owl#includes"/>
        <rdfs:domain rdf:resource="http://purl.org/ppeo/MDO.owl#object"/>
        <rdfs:range rdf:resource="http://purl.org/ppeo/MDO.owl#metadata_entity"/>
        <rdfs:comment xml:lang="en">Indicates that the parent object must include exactly one child entity.</rdfs:comment>
        <rdfs:label xml:lang="en">includes exactly one</rdfs:label>
    </owl:ObjectProperty>
    


    <!-- http://purl.org/ppeo/MDO.owl#includesMoreThanOne -->

    <owl:ObjectProperty rdf:about="http://purl.org/ppeo/MDO.owl#includesMoreThanOne">
        <rdfs:subPropertyOf rdf:resource="http://purl.org/ppeo/MDO.owl#includes"/>
        <rdfs:domain rdf:resource="http://purl.org/ppeo/MDO.owl#object"/>
        <rdfs:range rdf:resource="http://purl.org/ppeo/MDO.owl#metadata_entity"/>
        <rdfs:comment xml:lang="en">Indicates that the parent object must include more than one child entity.</rdfs:comment>
        <rdfs:label xml:lang="en">includes more than one</rdfs:label>
    </owl:ObjectProperty>
    


    <!-- http://purl.org/ppeo/MDO.owl#references -->

    <owl:ObjectProperty rdf:about="http://purl.org/ppeo/MDO.owl#references">
        <rdfs:domain rdf:resource="http://purl.org/ppeo/MDO.owl#selection_field"/>
        <rdfs:range rdf:resource="http://purl.org/ppeo/MDO.owl#list_field"/>
        <rdfs:comment xml:lang="en">Connects a selection field to a list field, the values of which will be the object of selection.</rdfs:comment>
        <rdfs:label xml:lang="en">references</rdfs:label>
    </owl:ObjectProperty>
    


    <!-- 
    ///////////////////////////////////////////////////////////////////////////////////////
    //
    // Data properties
    //
    ///////////////////////////////////////////////////////////////////////////////////////
     -->

    


    <!-- http://purl.org/ppeo/MDO.owl#from_list -->

    <owl:DatatypeProperty rdf:about="http://purl.org/ppeo/MDO.owl#from_list">
        <rdfs:domain>
            <owl:Class>
                <owl:unionOf rdf:parseType="Collection">
                    <rdf:Description rdf:about="http://purl.org/ppeo/MDO.owl#multiple_choice_field"/>
                    <rdf:Description rdf:about="http://purl.org/ppeo/MDO.owl#selection_field"/>
                </owl:unionOf>
            </owl:Class>
        </rdfs:domain>
        <rdfs:range rdf:resource="http://www.w3.org/2001/XMLSchema#string"/>
        <rdfs:comment xml:lang="en">Specifies a comma-separated list of possible values for a selection field.
The enumerated values can be specified, for example, as {&apos;value1&apos;, &apos;value2&apos;}.</rdfs:comment>
        <rdfs:label xml:lang="en">from list</rdfs:label>
    </owl:DatatypeProperty>
    


    <!-- http://purl.org/ppeo/MDO.owl#from_ontology -->

    <owl:DatatypeProperty rdf:about="http://purl.org/ppeo/MDO.owl#from_ontology">
        <rdfs:domain rdf:resource="http://purl.org/ppeo/MDO.owl#ontology_class_field"/>
        <rdfs:range rdf:resource="http://www.w3.org/2001/XMLSchema#anyURI"/>
        <rdfs:comment xml:lang="en">Indicates an ontology recommendation for an ontology class field, which can be the URI of an ontology or of a specific ontology class.</rdfs:comment>
        <rdfs:label xml:lang="en">from ontology</rdfs:label>
    </owl:DatatypeProperty>
    


    <!-- http://purl.org/ppeo/MDO.owl#from_vocabulary -->

    <owl:DatatypeProperty rdf:about="http://purl.org/ppeo/MDO.owl#from_vocabulary">
        <rdfs:domain rdf:resource="http://purl.org/ppeo/MDO.owl#controlled_vocabulary_field"/>
        <rdfs:range>
            <rdfs:Datatype>
                <owl:unionOf rdf:parseType="Collection">
                    <rdf:Description rdf:about="http://www.w3.org/2001/XMLSchema#anyURI"/>
                    <rdf:Description rdf:about="http://www.w3.org/2001/XMLSchema#string"/>
                </owl:unionOf>
            </rdfs:Datatype>
        </rdfs:range>
        <rdfs:comment xml:lang="en">Indicates a controlled vocabulary recommendation for a controlled vocabulary field.</rdfs:comment>
        <rdfs:label xml:lang="en">from vocabulary</rdfs:label>
    </owl:DatatypeProperty>
    


    <!-- http://purl.org/ppeo/MDO.owl#hasDefinition -->

    <owl:DatatypeProperty rdf:about="http://purl.org/ppeo/MDO.owl#hasDefinition">
        <rdf:type rdf:resource="http://www.w3.org/2002/07/owl#FunctionalProperty"/>
        <rdfs:domain rdf:resource="http://purl.org/ppeo/MDO.owl#metadata_entity"/>
        <rdfs:range rdf:resource="http://www.w3.org/2001/XMLSchema#string"/>
        <rdfs:comment xml:lang="en">Provides a human-readable definition for a metadata entity that may be displayed in the user interface to provide context for the user.</rdfs:comment>
        <rdfs:label xml:lang="en">has definition</rdfs:label>
    </owl:DatatypeProperty>
    


    <!-- http://purl.org/ppeo/MDO.owl#hasDisplayName -->

    <owl:DatatypeProperty rdf:about="http://purl.org/ppeo/MDO.owl#hasDisplayName">
        <rdf:type rdf:resource="http://www.w3.org/2002/07/owl#FunctionalProperty"/>
        <rdfs:domain rdf:resource="http://purl.org/ppeo/MDO.owl#metadata_entity"/>
        <rdfs:range rdf:resource="http://www.w3.org/2001/XMLSchema#string"/>
        <rdfs:comment xml:lang="en">The name of the metadata entity that will be shown on the interface.</rdfs:comment>
        <rdfs:label xml:lang="en">has display name</rdfs:label>
    </owl:DatatypeProperty>
    


    <!-- http://purl.org/ppeo/MDO.owl#hasExample -->

    <owl:DatatypeProperty rdf:about="http://purl.org/ppeo/MDO.owl#hasExample">
        <rdfs:domain rdf:resource="http://purl.org/ppeo/MDO.owl#field"/>
        <rdfs:range rdf:resource="http://www.w3.org/2001/XMLSchema#string"/>
        <rdfs:comment xml:lang="en">Provides an example value for a field, to assist the user in filling it in.</rdfs:comment>
        <rdfs:label xml:lang="en">has example</rdfs:label>
    </owl:DatatypeProperty>
    


    <!-- http://purl.org/ppeo/MDO.owl#hasOrderFactor -->

    <owl:DatatypeProperty rdf:about="http://purl.org/ppeo/MDO.owl#hasOrderFactor">
        <rdfs:domain rdf:resource="http://purl.org/ppeo/MDO.owl#metadata_entity"/>
        <rdfs:range rdf:resource="http://www.w3.org/2001/XMLSchema#integer"/>
        <rdfs:comment xml:lang="en">Assigns a number to a metadata entity that bears on the order in which it will be displayed within the containing/including metadata entity. Entities will be sorted by this number from lowest to highest.</rdfs:comment>
        <rdfs:label xml:lang="en">has order factor</rdfs:label>
    </owl:DatatypeProperty>
    


    <!-- http://purl.org/ppeo/MDO.owl#has_pattern -->

    <owl:DatatypeProperty rdf:about="http://purl.org/ppeo/MDO.owl#has_pattern">
        <rdfs:domain rdf:resource="http://purl.org/ppeo/MDO.owl#pattern_field"/>
        <rdfs:range rdf:resource="http://www.w3.org/2001/XMLSchema#string"/>
        <rdfs:comment xml:lang="en">Specifies a pattern to be used in a pattern field, using a standard regular expression (e.g. &apos;[0-9]{5}(-[0-9]{4})?&apos;).</rdfs:comment>
        <rdfs:label xml:lang="en">has pattern</rdfs:label>
    </owl:DatatypeProperty>
    


    <!-- http://purl.org/ppeo/MDO.owl#is_primary_key -->

    <owl:DatatypeProperty rdf:about="http://purl.org/ppeo/MDO.owl#is_primary_key">
        <rdf:type rdf:resource="http://www.w3.org/2002/07/owl#FunctionalProperty"/>
        <rdfs:domain rdf:resource="http://purl.org/ppeo/MDO.owl#field"/>
        <rdfs:range rdf:resource="http://www.w3.org/2001/XMLSchema#boolean"/>
        <rdfs:comment xml:lang="en">Specifies whether a field is the primary key for the containing object. If it is, then values for that field must be unique within the superobject that contains the object for which the field is the primary key. It will also be used as the identifier for the containing object, whenever it would be the target of a selection.
Primary keys cannot be optional.</rdfs:comment>
        <rdfs:label xml:lang="en">is primary key</rdfs:label>
    </owl:DatatypeProperty>
    


    <!-- 
    ///////////////////////////////////////////////////////////////////////////////////////
    //
    // Classes
    //
    ///////////////////////////////////////////////////////////////////////////////////////
     -->

    


    <!-- http://purl.org/ppeo/MDO.owl#URI_field -->

    <owl:Class rdf:about="http://purl.org/ppeo/MDO.owl#URI_field">
        <rdfs:subClassOf rdf:resource="http://purl.org/ppeo/MDO.owl#field"/>
        <rdfs:comment xml:lang="en">A field where a URI must be entered.</rdfs:comment>
        <rdfs:label xml:lang="en">URI field</rdfs:label>
    </owl:Class>
    


    <!-- http://purl.org/ppeo/MDO.owl#abstract_object -->

    <owl:Class rdf:about="http://purl.org/ppeo/MDO.owl#abstract_object">
        <rdfs:subClassOf rdf:resource="http://purl.org/ppeo/MDO.owl#object"/>
        <rdfs:subClassOf>
            <owl:Class>
                <owl:unionOf rdf:parseType="Collection">
                    <owl:Restriction>
                        <owl:onProperty rdf:resource="http://purl.org/ppeo/MDO.owl#contains"/>
                        <owl:someValuesFrom rdf:resource="http://purl.org/ppeo/MDO.owl#field"/>
                    </owl:Restriction>
                    <owl:Restriction>
                        <owl:onProperty rdf:resource="http://purl.org/ppeo/MDO.owl#includes"/>
                        <owl:someValuesFrom rdf:resource="http://purl.org/ppeo/MDO.owl#field"/>
                    </owl:Restriction>
                </owl:unionOf>
            </owl:Class>
        </rdfs:subClassOf>
        <rdfs:subClassOf>
            <owl:Restriction>
                <owl:onProperty rdf:resource="http://purl.org/ppeo/MDO.owl#contains"/>
                <owl:allValuesFrom rdf:resource="http://purl.org/ppeo/MDO.owl#field"/>
            </owl:Restriction>
        </rdfs:subClassOf>
        <rdfs:subClassOf>
            <owl:Restriction>
                <owl:onProperty rdf:resource="http://purl.org/ppeo/MDO.owl#includes"/>
                <owl:allValuesFrom rdf:resource="http://purl.org/ppeo/MDO.owl#field"/>
            </owl:Restriction>
        </rdfs:subClassOf>
        <owl:disjointWith rdf:resource="http://purl.org/ppeo/MDO.owl#section"/>
        <rdfs:comment xml:lang="en">An entity that requires (typically multiple) fields to describe.</rdfs:comment>
        <rdfs:label xml:lang="en">abstract object</rdfs:label>
    </owl:Class>
    


    <!-- http://purl.org/ppeo/MDO.owl#boolean_field -->

    <owl:Class rdf:about="http://purl.org/ppeo/MDO.owl#boolean_field">
        <rdfs:subClassOf rdf:resource="http://purl.org/ppeo/MDO.owl#field"/>
        <rdfs:comment xml:lang="en">A field where a boolean value must be entered.</rdfs:comment>
        <rdfs:label xml:lang="en">boolean field</rdfs:label>
    </owl:Class>
    


    <!-- http://purl.org/ppeo/MDO.owl#code_field -->

    <owl:Class rdf:about="http://purl.org/ppeo/MDO.owl#code_field">
        <rdfs:subClassOf rdf:resource="http://purl.org/ppeo/MDO.owl#field"/>
        <rdfs:comment xml:lang="en">A field where a (locally) unique identifier is expected. If left empty, the interface will generate a 16-character alphanumeric string upon export/save.</rdfs:comment>
        <rdfs:label xml:lang="en">code field</rdfs:label>
    </owl:Class>
    


    <!-- http://purl.org/ppeo/MDO.owl#controlled_vocabulary_field -->

    <owl:Class rdf:about="http://purl.org/ppeo/MDO.owl#controlled_vocabulary_field">
        <owl:equivalentClass>
            <owl:Class>
                <owl:intersectionOf rdf:parseType="Collection">
                    <rdf:Description rdf:about="http://purl.org/ppeo/MDO.owl#field"/>
                    <owl:Restriction>
                        <owl:onProperty rdf:resource="http://purl.org/ppeo/MDO.owl#from_vocabulary"/>
                        <owl:someValuesFrom>
                            <rdfs:Datatype>
                                <owl:unionOf rdf:parseType="Collection">
                                    <rdf:Description rdf:about="http://www.w3.org/2001/XMLSchema#anyURI"/>
                                    <rdf:Description rdf:about="http://www.w3.org/2001/XMLSchema#string"/>
                                </owl:unionOf>
                            </rdfs:Datatype>
                        </owl:someValuesFrom>
                    </owl:Restriction>
                </owl:intersectionOf>
            </owl:Class>
        </owl:equivalentClass>
        <rdfs:comment xml:lang="en">A field that is expected to take values from a recommended controlled vocabulary that is not available through an ontology lookup service, and therefore has to be manually searched by the user.</rdfs:comment>
        <rdfs:label xml:lang="en">controlled vocabulary field</rdfs:label>
    </owl:Class>
    


    <!-- http://purl.org/ppeo/MDO.owl#date_field -->

    <owl:Class rdf:about="http://purl.org/ppeo/MDO.owl#date_field">
        <rdfs:subClassOf rdf:resource="http://purl.org/ppeo/MDO.owl#field"/>
        <rdfs:comment xml:lang="en">A field where a date must be entered.</rdfs:comment>
        <rdfs:label xml:lang="en">date field</rdfs:label>
    </owl:Class>
    


    <!-- http://purl.org/ppeo/MDO.owl#field -->

    <owl:Class rdf:about="http://purl.org/ppeo/MDO.owl#field">
        <rdfs:subClassOf rdf:resource="http://purl.org/ppeo/MDO.owl#metadata_entity"/>
        <owl:disjointWith rdf:resource="http://purl.org/ppeo/MDO.owl#object"/>
        <rdfs:comment xml:lang="en">A metadata field (or attribute) for which the user is expected to enter or select a value. It should not be directly instantiated. A metadata field (or attribute) for which the user is expected to enter or select a value. It should not be directly instantiated.</rdfs:comment>
        <rdfs:label xml:lang="en">field</rdfs:label>
    </owl:Class>
    


    <!-- http://purl.org/ppeo/MDO.owl#float_field -->

    <owl:Class rdf:about="http://purl.org/ppeo/MDO.owl#float_field">
        <rdfs:subClassOf rdf:resource="http://purl.org/ppeo/MDO.owl#field"/>
        <rdfs:comment xml:lang="en">A field where a floating point value must be entered.</rdfs:comment>
        <rdfs:label xml:lang="en">float field</rdfs:label>
    </owl:Class>
    


    <!-- http://purl.org/ppeo/MDO.owl#free_text_field -->

    <owl:Class rdf:about="http://purl.org/ppeo/MDO.owl#free_text_field">
        <rdfs:subClassOf rdf:resource="http://purl.org/ppeo/MDO.owl#field"/>
        <rdfs:comment xml:lang="en">A field where (short) free text must be entered.</rdfs:comment>
        <rdfs:label xml:lang="en">free text field</rdfs:label>
    </owl:Class>
    


    <!-- http://purl.org/ppeo/MDO.owl#integer_field -->

    <owl:Class rdf:about="http://purl.org/ppeo/MDO.owl#integer_field">
        <rdfs:subClassOf rdf:resource="http://purl.org/ppeo/MDO.owl#field"/>
        <rdfs:comment xml:lang="en">A field where an integer value must be entered.</rdfs:comment>
        <rdfs:label xml:lang="en">integer field</rdfs:label>
    </owl:Class>
    


    <!-- http://purl.org/ppeo/MDO.owl#list_field -->

    <owl:Class rdf:about="http://purl.org/ppeo/MDO.owl#list_field">
        <rdfs:subClassOf rdf:resource="http://purl.org/ppeo/MDO.owl#field"/>
        <rdfs:comment xml:lang="en">A field where a list of values is expected, typically used to enumerate possible values an object can have.</rdfs:comment>
        <rdfs:label xml:lang="en">list field</rdfs:label>
    </owl:Class>
    


    <!-- http://purl.org/ppeo/MDO.owl#long_text_field -->

    <owl:Class rdf:about="http://purl.org/ppeo/MDO.owl#long_text_field">
        <rdfs:subClassOf rdf:resource="http://purl.org/ppeo/MDO.owl#field"/>
        <rdfs:comment xml:lang="en">A field where long free text can be entered, typically used for detailed descriptions.</rdfs:comment>
        <rdfs:label xml:lang="en">long text field</rdfs:label>
    </owl:Class>
    


    <!-- http://purl.org/ppeo/MDO.owl#metadata_entity -->

    <owl:Class rdf:about="http://purl.org/ppeo/MDO.owl#metadata_entity">
        <rdfs:comment xml:lang="en">A metadata entity, which can be a field or an object. It should not be directly instantiated.</rdfs:comment>
        <rdfs:label xml:lang="en">metadata entity</rdfs:label>
    </owl:Class>
    


    <!-- http://purl.org/ppeo/MDO.owl#multiple_choice_field -->

    <owl:Class rdf:about="http://purl.org/ppeo/MDO.owl#multiple_choice_field">
        <rdfs:subClassOf rdf:resource="http://purl.org/ppeo/MDO.owl#selection_field"/>
        <rdfs:comment xml:lang="en">A selection field where the user can select several values from among those listed.</rdfs:comment>
        <rdfs:label xml:lang="en">multiple choice field</rdfs:label>
    </owl:Class>
    


    <!-- http://purl.org/ppeo/MDO.owl#object -->

    <owl:Class rdf:about="http://purl.org/ppeo/MDO.owl#object">
        <rdfs:subClassOf rdf:resource="http://purl.org/ppeo/MDO.owl#metadata_entity"/>
        <rdfs:comment xml:lang="en">An entity that requires (typically multiple) fields to describe. It may also contain other sub-objects. It should not be directly instantiated</rdfs:comment>
        <rdfs:label xml:lang="en">object</rdfs:label>
    </owl:Class>
    


    <!-- http://purl.org/ppeo/MDO.owl#ontology_class_field -->

    <owl:Class rdf:about="http://purl.org/ppeo/MDO.owl#ontology_class_field">
        <owl:equivalentClass>
            <owl:Class>
                <owl:intersectionOf rdf:parseType="Collection">
                    <rdf:Description rdf:about="http://purl.org/ppeo/MDO.owl#field"/>
                    <owl:Restriction>
                        <owl:onProperty rdf:resource="http://purl.org/ppeo/MDO.owl#from_ontology"/>
                        <owl:someValuesFrom rdf:resource="http://www.w3.org/2001/XMLSchema#anyURI"/>
                    </owl:Restriction>
                </owl:intersectionOf>
            </owl:Class>
        </owl:equivalentClass>
        <rdfs:comment xml:lang="en">A field that is expected to take as value a class from among those in one or more given ontologies or from the subclasses of one or more given ontology class, listed through the &apos;from ontology&apos; property. Ontology classes should be searched using an ontology lookup service. Free-text values can be accepted if no suitable ontology concepts exist.</rdfs:comment>
        <rdfs:label xml:lang="en">ontology class field</rdfs:label>
    </owl:Class>
    


    <!-- http://purl.org/ppeo/MDO.owl#pattern_field -->

    <owl:Class rdf:about="http://purl.org/ppeo/MDO.owl#pattern_field">
        <owl:equivalentClass>
            <owl:Class>
                <owl:intersectionOf rdf:parseType="Collection">
                    <rdf:Description rdf:about="http://purl.org/ppeo/MDO.owl#field"/>
                    <owl:Restriction>
                        <owl:onProperty rdf:resource="http://purl.org/ppeo/MDO.owl#has_pattern"/>
                        <owl:someValuesFrom rdf:resource="http://www.w3.org/2001/XMLSchema#string"/>
                    </owl:Restriction>
                </owl:intersectionOf>
            </owl:Class>
        </owl:equivalentClass>
        <rdfs:comment xml:lang="en">A field where a string must be entered that matches a specified pattern, provided using the property &apos;has pattern&apos;.</rdfs:comment>
        <rdfs:label xml:lang="en">pattern field</rdfs:label>
    </owl:Class>
    


    <!-- http://purl.org/ppeo/MDO.owl#section -->

    <owl:Class rdf:about="http://purl.org/ppeo/MDO.owl#section">
        <rdfs:subClassOf rdf:resource="http://purl.org/ppeo/MDO.owl#object"/>
        <rdfs:subClassOf>
            <owl:Class>
                <owl:unionOf rdf:parseType="Collection">
                    <owl:Restriction>
                        <owl:onProperty rdf:resource="http://purl.org/ppeo/MDO.owl#contains"/>
                        <owl:someValuesFrom rdf:resource="http://purl.org/ppeo/MDO.owl#metadata_entity"/>
                    </owl:Restriction>
                    <owl:Restriction>
                        <owl:onProperty rdf:resource="http://purl.org/ppeo/MDO.owl#includes"/>
                        <owl:someValuesFrom rdf:resource="http://purl.org/ppeo/MDO.owl#metadata_entity"/>
                    </owl:Restriction>
                </owl:unionOf>
            </owl:Class>
        </rdfs:subClassOf>
        <rdfs:comment xml:lang="en">An object that should be visualized on its own, typically because it contains numerous fields or sub-objects and/or because it represents a conceptually independent portion of a metadata scheme.</rdfs:comment>
        <rdfs:label xml:lang="en">section</rdfs:label>
    </owl:Class>
    


    <!-- http://purl.org/ppeo/MDO.owl#selection_field -->

    <owl:Class rdf:about="http://purl.org/ppeo/MDO.owl#selection_field">
        <owl:equivalentClass>
            <owl:Class>
                <owl:intersectionOf rdf:parseType="Collection">
                    <rdf:Description rdf:about="http://purl.org/ppeo/MDO.owl#field"/>
                    <owl:Class>
                        <owl:unionOf rdf:parseType="Collection">
                            <owl:Restriction>
                                <owl:onProperty rdf:resource="http://purl.org/ppeo/MDO.owl#references"/>
                                <owl:someValuesFrom rdf:resource="http://purl.org/ppeo/MDO.owl#list_field"/>
                            </owl:Restriction>
                            <owl:Restriction>
                                <owl:onProperty rdf:resource="http://purl.org/ppeo/MDO.owl#from_list"/>
                                <owl:someValuesFrom rdf:resource="http://www.w3.org/2001/XMLSchema#string"/>
                            </owl:Restriction>
                        </owl:unionOf>
                    </owl:Class>
                </owl:intersectionOf>
            </owl:Class>
        </owl:equivalentClass>
        <rdfs:comment xml:lang="en">A field where the user is expected to select from among a list of possible values. This list can either be a list field linked through the &apos;references&apos; property (note the list field must have been filled before the selection is made), or a fixed list provided through the property &apos;from list&apos;. If pointing to a list field that has plural cardinality, the user should be first asked to select an instance of that  field, identified by the containing objectâ€™s primary field if applicable.</rdfs:comment>
        <rdfs:label xml:lang="en">selection field</rdfs:label>
    </owl:Class>
    


    <!-- http://purl.org/ppeo/MDO.owl#single_choice_field -->

    <owl:Class rdf:about="http://purl.org/ppeo/MDO.owl#single_choice_field">
        <rdfs:subClassOf rdf:resource="http://purl.org/ppeo/MDO.owl#selection_field"/>
        <rdfs:comment xml:lang="en">A selection field where the user can only select one value from among those listed.</rdfs:comment>
        <rdfs:label xml:lang="en">single choice field</rdfs:label>
    </owl:Class>
    


    <!-- http://purl.org/ppeo/MDO.owl#top_section -->

    <owl:Class rdf:about="http://purl.org/ppeo/MDO.owl#top_section">
        <owl:equivalentClass>
            <owl:Class>
                <owl:intersectionOf rdf:parseType="Collection">
                    <rdf:Description rdf:about="http://purl.org/ppeo/MDO.owl#section"/>
                    <owl:Restriction>
                        <owl:onProperty>
                            <rdf:Description>
                                <owl:inverseOf rdf:resource="http://purl.org/ppeo/MDO.owl#contains"/>
                            </rdf:Description>
                        </owl:onProperty>
                        <owl:maxQualifiedCardinality rdf:datatype="http://www.w3.org/2001/XMLSchema#nonNegativeInteger">0</owl:maxQualifiedCardinality>
                        <owl:onClass rdf:resource="http://purl.org/ppeo/MDO.owl#object"/>
                    </owl:Restriction>
                </owl:intersectionOf>
            </owl:Class>
        </owl:equivalentClass>
        <rdfs:comment xml:lang="en">The topmost entity in the metadata schema, containing all other sections, objects and fields.</rdfs:comment>
        <rdfs:label xml:lang="en">top section</rdfs:label>
    </owl:Class>
</rdf:RDF>



<!-- Generated by the OWL API (version 4.5.9.2019-02-01T07:24:44Z) https://github.com/owlcs/owlapi -->

