<?xml version="1.0"?>
<rdf:RDF xmlns="http://purl.org/ppeo/MDO.owl#"
     xml:base="http://purl.org/ppeo/MDO.owl"
     xmlns:owl="http://www.w3.org/2002/07/owl#"
     xmlns:rdf="http://www.w3.org/1999/02/22-rdf-syntax-ns#"
     xmlns:xml="http://www.w3.org/XML/1998/namespace"
     xmlns:xsd="http://www.w3.org/2001/XMLSchema#"
     xmlns:rdfs="http://www.w3.org/2000/01/rdf-schema#">
    <owl:Ontology rdf:about="http://purl.org/ppeo/MDO.owl"/>
    


    <!-- 
    ///////////////////////////////////////////////////////////////////////////////////////
    //
    // Object Properties
    //
    ///////////////////////////////////////////////////////////////////////////////////////
     -->

    


    <!-- http://purl.org/ppeo/MDO.owl#contains -->

    <owl:ObjectProperty rdf:about="http://purl.org/ppeo/MDO.owl#contains">
        <rdfs:domain rdf:resource="http://purl.org/ppeo/MDO.owl#object"/>
        <rdfs:range>
            <owl:Class>
                <owl:unionOf rdf:parseType="Collection">
                    <rdf:Description rdf:about="http://purl.org/ppeo/MDO.owl#field"/>
                    <rdf:Description rdf:about="http://purl.org/ppeo/MDO.owl#object"/>
                </owl:unionOf>
            </owl:Class>
        </rdfs:range>
        <rdfs:comment xml:lang="en">Expresses a whole-part relation between an object and another object or field which should be reflected in the structure of the interface.</rdfs:comment>
        <rdfs:label xml:lang="en">contains</rdfs:label>
    </owl:ObjectProperty>
    


    <!-- http://purl.org/ppeo/MDO.owl#containsAtLeastOne -->

    <owl:ObjectProperty rdf:about="http://purl.org/ppeo/MDO.owl#containsAtLeastOne">
        <rdfs:subPropertyOf rdf:resource="http://purl.org/ppeo/MDO.owl#contains"/>
        <rdfs:domain rdf:resource="http://purl.org/ppeo/MDO.owl#object"/>
        <rdfs:range>
            <owl:Class>
                <owl:unionOf rdf:parseType="Collection">
                    <rdf:Description rdf:about="http://purl.org/ppeo/MDO.owl#field"/>
                    <rdf:Description rdf:about="http://purl.org/ppeo/MDO.owl#object"/>
                </owl:unionOf>
            </owl:Class>
        </rdfs:range>
        <rdfs:comment xml:lang="en">Indicates that the parent object must contain at least one of the children.</rdfs:comment>
        <rdfs:label xml:lang="en">contains at least one</rdfs:label>
    </owl:ObjectProperty>
    


    <!-- http://purl.org/ppeo/MDO.owl#containsAtMostOne -->

    <owl:ObjectProperty rdf:about="http://purl.org/ppeo/MDO.owl#containsAtMostOne">
        <rdfs:subPropertyOf rdf:resource="http://purl.org/ppeo/MDO.owl#contains"/>
        <rdfs:domain rdf:resource="http://purl.org/ppeo/MDO.owl#object"/>
        <rdfs:range>
            <owl:Class>
                <owl:unionOf rdf:parseType="Collection">
                    <rdf:Description rdf:about="http://purl.org/ppeo/MDO.owl#field"/>
                    <rdf:Description rdf:about="http://purl.org/ppeo/MDO.owl#object"/>
                </owl:unionOf>
            </owl:Class>
        </rdfs:range>
        <rdfs:comment xml:lang="en">Indicates that the parent object can contain at most one children.</rdfs:comment>
        <rdfs:label xml:lang="en">contains at most one</rdfs:label>
    </owl:ObjectProperty>
    


    <!-- http://purl.org/ppeo/MDO.owl#containsExactlyOne -->

    <owl:ObjectProperty rdf:about="http://purl.org/ppeo/MDO.owl#containsExactlyOne">
        <rdfs:subPropertyOf rdf:resource="http://purl.org/ppeo/MDO.owl#contains"/>
        <rdfs:domain rdf:resource="http://purl.org/ppeo/MDO.owl#object"/>
        <rdfs:range>
            <owl:Class>
                <owl:unionOf rdf:parseType="Collection">
                    <rdf:Description rdf:about="http://purl.org/ppeo/MDO.owl#field"/>
                    <rdf:Description rdf:about="http://purl.org/ppeo/MDO.owl#object"/>
                </owl:unionOf>
            </owl:Class>
        </rdfs:range>
        <rdfs:comment xml:lang="en">Indicates that the parent object must contain exactly one of the children.</rdfs:comment>
        <rdfs:label xml:lang="en">contains exactly one</rdfs:label>
    </owl:ObjectProperty>
    


    <!-- http://purl.org/ppeo/MDO.owl#containsMoreThanOne -->

    <owl:ObjectProperty rdf:about="http://purl.org/ppeo/MDO.owl#containsMoreThanOne">
        <rdfs:subPropertyOf rdf:resource="http://purl.org/ppeo/MDO.owl#contains"/>
        <rdfs:domain rdf:resource="http://purl.org/ppeo/MDO.owl#object"/>
        <rdfs:range>
            <owl:Class>
                <owl:unionOf rdf:parseType="Collection">
                    <rdf:Description rdf:about="http://purl.org/ppeo/MDO.owl#field"/>
                    <rdf:Description rdf:about="http://purl.org/ppeo/MDO.owl#object"/>
                </owl:unionOf>
            </owl:Class>
        </rdfs:range>
        <rdfs:comment xml:lang="en">Indicates that the parent object must contain more than one of the children.</rdfs:comment>
        <rdfs:label xml:lang="en">contains more than one</rdfs:label>
    </owl:ObjectProperty>
    


    <!-- http://purl.org/ppeo/MDO.owl#hasNext -->

    <owl:ObjectProperty rdf:about="http://purl.org/ppeo/MDO.owl#hasNext">
        <rdf:type rdf:resource="http://www.w3.org/2002/07/owl#FunctionalProperty"/>
        <rdfs:domain>
            <owl:Class>
                <owl:unionOf rdf:parseType="Collection">
                    <rdf:Description rdf:about="http://purl.org/ppeo/MDO.owl#field"/>
                    <rdf:Description rdf:about="http://purl.org/ppeo/MDO.owl#object"/>
                </owl:unionOf>
            </owl:Class>
        </rdfs:domain>
        <rdfs:range>
            <owl:Class>
                <owl:unionOf rdf:parseType="Collection">
                    <rdf:Description rdf:about="http://purl.org/ppeo/MDO.owl#field"/>
                    <rdf:Description rdf:about="http://purl.org/ppeo/MDO.owl#object"/>
                </owl:unionOf>
            </owl:Class>
        </rdfs:range>
        <rdfs:comment xml:lang="en">Used to create a chain of fields/sections/objects to define the display order of elements in the interface.</rdfs:comment>
        <rdfs:label xml:lang="en">next</rdfs:label>
    </owl:ObjectProperty>
    


    <!-- http://purl.org/ppeo/MDO.owl#includes -->

    <owl:ObjectProperty rdf:about="http://purl.org/ppeo/MDO.owl#includes">
        <rdfs:comment xml:lang="en">Expresses a connection between the current parent and an existing child.</rdfs:comment>
        <rdfs:label xml:lang="en">includes</rdfs:label>
    </owl:ObjectProperty>
    


    <!-- http://purl.org/ppeo/MDO.owl#includesAtLeastOne -->

    <owl:ObjectProperty rdf:about="http://purl.org/ppeo/MDO.owl#includesAtLeastOne">
        <rdfs:subPropertyOf rdf:resource="http://purl.org/ppeo/MDO.owl#includes"/>
        <rdfs:label xml:lang="en">includes at least one</rdfs:label>
    </owl:ObjectProperty>
    


    <!-- http://purl.org/ppeo/MDO.owl#includesAtMostOne -->

    <owl:ObjectProperty rdf:about="http://purl.org/ppeo/MDO.owl#includesAtMostOne">
        <rdfs:subPropertyOf rdf:resource="http://purl.org/ppeo/MDO.owl#includes"/>
        <rdfs:label xml:lang="en">includes at most one</rdfs:label>
    </owl:ObjectProperty>
    


    <!-- http://purl.org/ppeo/MDO.owl#includesExactlyOne -->

    <owl:ObjectProperty rdf:about="http://purl.org/ppeo/MDO.owl#includesExactlyOne">
        <rdfs:subPropertyOf rdf:resource="http://purl.org/ppeo/MDO.owl#includes"/>
        <rdfs:label xml:lang="en">includes exactly one</rdfs:label>
    </owl:ObjectProperty>
    


    <!-- http://purl.org/ppeo/MDO.owl#includesMoreThanOne -->

    <owl:ObjectProperty rdf:about="http://purl.org/ppeo/MDO.owl#includesMoreThanOne">
        <rdfs:subPropertyOf rdf:resource="http://purl.org/ppeo/MDO.owl#includes"/>
        <rdfs:label xml:lang="en">includes more than one</rdfs:label>
    </owl:ObjectProperty>
    


    <!-- http://purl.org/ppeo/MDO.owl#references -->

    <owl:ObjectProperty rdf:about="http://purl.org/ppeo/MDO.owl#references">
        <rdfs:domain rdf:resource="http://purl.org/ppeo/MDO.owl#selection_field"/>
        <rdfs:range rdf:resource="http://purl.org/ppeo/MDO.owl#enumeration_field"/>
        <rdfs:comment xml:lang="en">Used to connect two fields, when a selection must be made from the object field (enumeration) for the subject field (selection field).</rdfs:comment>
        <rdfs:label xml:lang="en">references</rdfs:label>
    </owl:ObjectProperty>
    


    <!-- 
    ///////////////////////////////////////////////////////////////////////////////////////
    //
    // Data properties
    //
    ///////////////////////////////////////////////////////////////////////////////////////
     -->

    


    <!-- http://purl.org/ppeo/MDO.owl#hasDataType -->

    <owl:DatatypeProperty rdf:about="http://purl.org/ppeo/MDO.owl#hasDataType">
        <rdfs:comment xml:lang="en">Indicates the type of data (e.g. string, number, date) that is expected in a Fixed datatype field. A pattern can also be defined using regular expressions (e.g. xsd:string[pattern &quot;[0-9]{5}(-[0-9]{4})?&quot;]).</rdfs:comment>
        <rdfs:label xml:lang="en">data type</rdfs:label>
    </owl:DatatypeProperty>
    


    <!-- http://purl.org/ppeo/MDO.owl#hasDefinition -->

    <owl:DatatypeProperty rdf:about="http://purl.org/ppeo/MDO.owl#hasDefinition">
        <rdf:type rdf:resource="http://www.w3.org/2002/07/owl#FunctionalProperty"/>
        <rdfs:domain>
            <owl:Class>
                <owl:unionOf rdf:parseType="Collection">
                    <rdf:Description rdf:about="http://purl.org/ppeo/MDO.owl#field"/>
                    <rdf:Description rdf:about="http://purl.org/ppeo/MDO.owl#object"/>
                </owl:unionOf>
            </owl:Class>
        </rdfs:domain>
        <rdfs:range rdf:resource="http://www.w3.org/2001/XMLSchema#string"/>
        <rdfs:comment xml:lang="en">Shows the definition for fields that the users have to fill in.</rdfs:comment>
        <rdfs:label xml:lang="en">definition</rdfs:label>
    </owl:DatatypeProperty>
    


    <!-- http://purl.org/ppeo/MDO.owl#hasDisplayName -->

    <owl:DatatypeProperty rdf:about="http://purl.org/ppeo/MDO.owl#hasDisplayName">
        <rdf:type rdf:resource="http://www.w3.org/2002/07/owl#FunctionalProperty"/>
        <rdfs:domain>
            <owl:Class>
                <owl:unionOf rdf:parseType="Collection">
                    <rdf:Description rdf:about="http://purl.org/ppeo/MDO.owl#field"/>
                    <rdf:Description rdf:about="http://purl.org/ppeo/MDO.owl#object"/>
                </owl:unionOf>
            </owl:Class>
        </rdfs:domain>
        <rdfs:range rdf:resource="http://www.w3.org/2001/XMLSchema#string"/>
        <rdfs:comment xml:lang="en">The name of the fields/section/object that will be shown on the interface.</rdfs:comment>
        <rdfs:label xml:lang="en">display name</rdfs:label>
    </owl:DatatypeProperty>
    


    <!-- http://purl.org/ppeo/MDO.owl#hasExample -->

    <owl:DatatypeProperty rdf:about="http://purl.org/ppeo/MDO.owl#hasExample">
        <rdfs:domain rdf:resource="http://purl.org/ppeo/MDO.owl#field"/>
        <rdfs:comment xml:lang="en">An example value for a field.</rdfs:comment>
        <rdfs:label xml:lang="en">example</rdfs:label>
    </owl:DatatypeProperty>
    


    <!-- http://purl.org/ppeo/MDO.owl#hasOntologyRecommendation -->

    <owl:DatatypeProperty rdf:about="http://purl.org/ppeo/MDO.owl#hasOntologyRecommendation">
        <rdfs:domain rdf:resource="http://purl.org/ppeo/MDO.owl#field"/>
        <rdfs:range>
            <rdfs:Datatype>
                <owl:unionOf rdf:parseType="Collection">
                    <rdf:Description rdf:about="http://www.w3.org/2001/XMLSchema#anyURI"/>
                    <rdf:Description rdf:about="http://www.w3.org/2001/XMLSchema#string"/>
                </owl:unionOf>
            </rdfs:Datatype>
        </rdfs:range>
        <rdfs:comment xml:lang="en">Can be used to point to ontologies / controlled vocabularies for a field.</rdfs:comment>
        <rdfs:label xml:lang="en">ontology recommendation</rdfs:label>
    </owl:DatatypeProperty>
    


    <!-- http://purl.org/ppeo/MDO.owl#isHead -->

    <owl:DatatypeProperty rdf:about="http://purl.org/ppeo/MDO.owl#isHead">
        <rdf:type rdf:resource="http://www.w3.org/2002/07/owl#FunctionalProperty"/>
        <rdfs:domain>
            <owl:Class>
                <owl:unionOf rdf:parseType="Collection">
                    <rdf:Description rdf:about="http://purl.org/ppeo/MDO.owl#field"/>
                    <rdf:Description rdf:about="http://purl.org/ppeo/MDO.owl#object"/>
                </owl:unionOf>
            </owl:Class>
        </rdfs:domain>
        <rdfs:range rdf:resource="http://www.w3.org/2001/XMLSchema#boolean"/>
        <rdfs:comment xml:lang="en">The first field to be shown in a section/object.</rdfs:comment>
        <rdfs:label xml:lang="en">head</rdfs:label>
    </owl:DatatypeProperty>
    


    <!-- http://purl.org/ppeo/MDO.owl#isTail -->

    <owl:DatatypeProperty rdf:about="http://purl.org/ppeo/MDO.owl#isTail">
        <rdfs:subPropertyOf rdf:resource="http://www.w3.org/2002/07/owl#topDataProperty"/>
        <rdfs:domain>
            <owl:Class>
                <owl:unionOf rdf:parseType="Collection">
                    <rdf:Description rdf:about="http://purl.org/ppeo/MDO.owl#field"/>
                    <rdf:Description rdf:about="http://purl.org/ppeo/MDO.owl#object"/>
                </owl:unionOf>
            </owl:Class>
        </rdfs:domain>
        <rdfs:range rdf:resource="http://www.w3.org/2001/XMLSchema#boolean"/>
        <rdfs:comment xml:lang="en">The last field to be shown in a section/object.</rdfs:comment>
        <rdfs:label xml:lang="en">tail</rdfs:label>
    </owl:DatatypeProperty>
    


    <!-- http://purl.org/ppeo/MDO.owl#isTopSection -->

    <owl:DatatypeProperty rdf:about="http://purl.org/ppeo/MDO.owl#isTopSection">
        <rdf:type rdf:resource="http://www.w3.org/2002/07/owl#FunctionalProperty"/>
        <rdfs:domain rdf:resource="http://purl.org/ppeo/MDO.owl#section"/>
        <rdfs:range rdf:resource="http://www.w3.org/2001/XMLSchema#boolean"/>
        <rdfs:comment xml:lang="en">Marks a section that has no parent.</rdfs:comment>
        <rdfs:label xml:lang="en">top section</rdfs:label>
    </owl:DatatypeProperty>
    


    <!-- 
    ///////////////////////////////////////////////////////////////////////////////////////
    //
    // Classes
    //
    ///////////////////////////////////////////////////////////////////////////////////////
     -->

    


    <!-- http://purl.org/ppeo/MDO.owl#ID_field -->

    <owl:Class rdf:about="http://purl.org/ppeo/MDO.owl#ID_field">
        <rdfs:subClassOf rdf:resource="http://purl.org/ppeo/MDO.owl#field"/>
        <rdfs:comment xml:lang="en">A field holding the main identifier for the resource being described.</rdfs:comment>
        <rdfs:label xml:lang="en">ID field</rdfs:label>
    </owl:Class>
    


    <!-- http://purl.org/ppeo/MDO.owl#controlled_vocabulary_field -->

    <owl:Class rdf:about="http://purl.org/ppeo/MDO.owl#controlled_vocabulary_field">
        <rdfs:subClassOf rdf:resource="http://purl.org/ppeo/MDO.owl#field"/>
        <rdfs:comment xml:lang="en">A field that is expected to take values from a recommended external ontology or controlled vocabulary, but also accepts free-text values if no suitable ontology concepts exist.</rdfs:comment>
        <rdfs:label xml:lang="en">controlled vocabulary field</rdfs:label>
    </owl:Class>
    


    <!-- http://purl.org/ppeo/MDO.owl#enumeration_field -->

    <owl:Class rdf:about="http://purl.org/ppeo/MDO.owl#enumeration_field">
        <rdfs:subClassOf rdf:resource="http://purl.org/ppeo/MDO.owl#field"/>
        <rdfs:comment xml:lang="en">A field that expects a list  of possible values. It can be paired with a selection field to allow the user to specify any number of those values elsewhere in the metadata structure.</rdfs:comment>
        <rdfs:label xml:lang="en">enumeration field</rdfs:label>
    </owl:Class>
    


    <!-- http://purl.org/ppeo/MDO.owl#field -->

    <owl:Class rdf:about="http://purl.org/ppeo/MDO.owl#field">
        <rdfs:comment xml:lang="en">A metadata field (or attribute) for which the user is expected to enter a value.</rdfs:comment>
        <rdfs:label xml:lang="en">field</rdfs:label>
    </owl:Class>
    


    <!-- http://purl.org/ppeo/MDO.owl#fixed_datatype_field -->

    <owl:Class rdf:about="http://purl.org/ppeo/MDO.owl#fixed_datatype_field">
        <rdfs:subClassOf rdf:resource="http://purl.org/ppeo/MDO.owl#field"/>
        <rdfs:comment xml:lang="en">A field where a specified value type is expected  (e.g. number, date).</rdfs:comment>
        <rdfs:label xml:lang="en">fixed datatype field</rdfs:label>
    </owl:Class>
    


    <!-- http://purl.org/ppeo/MDO.owl#free_value_field -->

    <owl:Class rdf:about="http://purl.org/ppeo/MDO.owl#free_value_field">
        <rdfs:subClassOf rdf:resource="http://purl.org/ppeo/MDO.owl#field"/>
        <rdfs:comment xml:lang="en">A field where any value can be entered without type restrictions but with expected short length.</rdfs:comment>
        <rdfs:label xml:lang="en">free value field</rdfs:label>
    </owl:Class>
    


    <!-- http://purl.org/ppeo/MDO.owl#long_text_field -->

    <owl:Class rdf:about="http://purl.org/ppeo/MDO.owl#long_text_field">
        <rdfs:subClassOf rdf:resource="http://purl.org/ppeo/MDO.owl#field"/>
        <rdfs:comment xml:lang="en">A field where long free text can be entered, typically used for detailed descriptions.</rdfs:comment>
        <rdfs:label xml:lang="en">long text field</rdfs:label>
    </owl:Class>
    


    <!-- http://purl.org/ppeo/MDO.owl#object -->

    <owl:Class rdf:about="http://purl.org/ppeo/MDO.owl#object">
        <rdfs:comment xml:lang="en">An entity that requires (typically multiple) fields to describe. It may also contain other sub-objects.</rdfs:comment>
        <rdfs:label xml:lang="en">object</rdfs:label>
    </owl:Class>
    


    <!-- http://purl.org/ppeo/MDO.owl#restriction_field -->

    <owl:Class rdf:about="http://purl.org/ppeo/MDO.owl#restriction_field">
        <rdfs:subClassOf rdf:resource="http://purl.org/ppeo/MDO.owl#selection_field"/>
        <rdfs:comment xml:lang="en">A field that can only take a single value from a specified enumeration field.</rdfs:comment>
        <rdfs:label xml:lang="en">restriction field</rdfs:label>
    </owl:Class>
    


    <!-- http://purl.org/ppeo/MDO.owl#section -->

    <owl:Class rdf:about="http://purl.org/ppeo/MDO.owl#section">
        <rdfs:subClassOf rdf:resource="http://purl.org/ppeo/MDO.owl#object"/>
        <rdfs:comment xml:lang="en">An object that should be visualized on its own, typically because it contains numerous fields or sub-objects and/or because it represents a conceptually independent portion of a metadata scheme.</rdfs:comment>
        <rdfs:label xml:lang="en">section</rdfs:label>
    </owl:Class>
    


    <!-- http://purl.org/ppeo/MDO.owl#selection_field -->

    <owl:Class rdf:about="http://purl.org/ppeo/MDO.owl#selection_field">
        <rdfs:subClassOf rdf:resource="http://purl.org/ppeo/MDO.owl#field"/>
        <rdfs:comment xml:lang="en">A field that can only take values from among those listed in a specified  enumeration field.</rdfs:comment>
        <rdfs:label xml:lang="en">selection field</rdfs:label>
    </owl:Class>
</rdf:RDF>



<!-- Generated by the OWL API (version 4.5.9.2019-02-01T07:24:44Z) https://github.com/owlcs/owlapi -->

