<?xml version="1.0"?>
<rdf:RDF xmlns="http://purl.org/ppeo/MDO.owl#"
     xml:base="http://purl.org/ppeo/MDO.owl"
     xmlns:owl="http://www.w3.org/2002/07/owl#"
     xmlns:rdf="http://www.w3.org/1999/02/22-rdf-syntax-ns#"
     xmlns:xml="http://www.w3.org/XML/1998/namespace"
     xmlns:xsd="http://www.w3.org/2001/XMLSchema#"
     xmlns:rdfs="http://www.w3.org/2000/01/rdf-schema#">
    <owl:Ontology rdf:about="http://purl.org/ppeo/MDO.owl"/>
    


    <!-- 
    ///////////////////////////////////////////////////////////////////////////////////////
    //
    // Object Properties
    //
    ///////////////////////////////////////////////////////////////////////////////////////
     -->

    


    <!-- http://purl.org/ppeo/MDO.owl#contains -->

    <owl:ObjectProperty rdf:about="http://purl.org/ppeo/MDO.owl#contains">
        <rdfs:domain rdf:resource="http://purl.org/ppeo/MDO.owl#object"/>
        <rdfs:range rdf:resource="http://purl.org/ppeo/MDO.owl#metadata_entity"/>
        <rdfs:comment xml:lang="en">Expresses a whole-part relation between an object and another object or field which should be reflected in the structure of the interface (e.g. contained fields should be displayed within the containing sections, and contained subsections should be englobed by or linked to their containing sections).</rdfs:comment>
        <rdfs:label xml:lang="en">contains</rdfs:label>
    </owl:ObjectProperty>
    


    <!-- http://purl.org/ppeo/MDO.owl#containsAtLeastOne -->

    <owl:ObjectProperty rdf:about="http://purl.org/ppeo/MDO.owl#containsAtLeastOne">
        <rdfs:subPropertyOf rdf:resource="http://purl.org/ppeo/MDO.owl#contains"/>
        <rdfs:domain rdf:resource="http://purl.org/ppeo/MDO.owl#object"/>
        <rdfs:range rdf:resource="http://purl.org/ppeo/MDO.owl#metadata_entity"/>
        <rdfs:comment xml:lang="en">Indicates that the parent object must contain at least one child entity.</rdfs:comment>
        <rdfs:label xml:lang="en">contains at least one</rdfs:label>
    </owl:ObjectProperty>
    


    <!-- http://purl.org/ppeo/MDO.owl#containsAtMostOne -->

    <owl:ObjectProperty rdf:about="http://purl.org/ppeo/MDO.owl#containsAtMostOne">
        <rdfs:subPropertyOf rdf:resource="http://purl.org/ppeo/MDO.owl#contains"/>
        <rdfs:domain rdf:resource="http://purl.org/ppeo/MDO.owl#object"/>
        <rdfs:range rdf:resource="http://purl.org/ppeo/MDO.owl#metadata_entity"/>
        <rdfs:comment xml:lang="en">Indicates that the parent object can contain at most one child entity.</rdfs:comment>
        <rdfs:label xml:lang="en">contains at most one</rdfs:label>
    </owl:ObjectProperty>
    


    <!-- http://purl.org/ppeo/MDO.owl#containsExactlyOne -->

    <owl:ObjectProperty rdf:about="http://purl.org/ppeo/MDO.owl#containsExactlyOne">
        <rdfs:subPropertyOf rdf:resource="http://purl.org/ppeo/MDO.owl#contains"/>
        <rdfs:domain rdf:resource="http://purl.org/ppeo/MDO.owl#object"/>
        <rdfs:range rdf:resource="http://purl.org/ppeo/MDO.owl#metadata_entity"/>
        <rdfs:comment xml:lang="en">Indicates that the parent object must contain exactly one child entity.</rdfs:comment>
        <rdfs:label xml:lang="en">contains exactly one</rdfs:label>
    </owl:ObjectProperty>
    


    <!-- http://purl.org/ppeo/MDO.owl#containsMoreThanOne -->

    <owl:ObjectProperty rdf:about="http://purl.org/ppeo/MDO.owl#containsMoreThanOne">
        <rdfs:subPropertyOf rdf:resource="http://purl.org/ppeo/MDO.owl#contains"/>
        <rdfs:domain rdf:resource="http://purl.org/ppeo/MDO.owl#object"/>
        <rdfs:range rdf:resource="http://purl.org/ppeo/MDO.owl#metadata_entity"/>
        <rdfs:comment xml:lang="en">Indicates that the parent object must contain more than one child entity.</rdfs:comment>
        <rdfs:label xml:lang="en">contains more than one</rdfs:label>
    </owl:ObjectProperty>
    


    <!-- http://purl.org/ppeo/MDO.owl#includes -->

    <owl:ObjectProperty rdf:about="http://purl.org/ppeo/MDO.owl#includes">
        <rdfs:domain rdf:resource="http://purl.org/ppeo/MDO.owl#object"/>
        <rdfs:range rdf:resource="http://purl.org/ppeo/MDO.owl#metadata_entity"/>
        <rdfs:comment xml:lang="en">Expresses a whole-part relation between an object and an entity that has been previously instanced, to allow the allocation of that instance to the parent object. This should be reflected in the interface displaying a selector of instances of the child object that have been previously entered elsewhere in this metadata form.</rdfs:comment>
        <rdfs:label xml:lang="en">includes</rdfs:label>
    </owl:ObjectProperty>
    


    <!-- http://purl.org/ppeo/MDO.owl#includesAtLeastOne -->

    <owl:ObjectProperty rdf:about="http://purl.org/ppeo/MDO.owl#includesAtLeastOne">
        <rdfs:subPropertyOf rdf:resource="http://purl.org/ppeo/MDO.owl#includes"/>
        <rdfs:domain rdf:resource="http://purl.org/ppeo/MDO.owl#object"/>
        <rdfs:range rdf:resource="http://purl.org/ppeo/MDO.owl#metadata_entity"/>
        <rdfs:label xml:lang="en">includes at least one</rdfs:label>
    </owl:ObjectProperty>
    


    <!-- http://purl.org/ppeo/MDO.owl#includesAtMostOne -->

    <owl:ObjectProperty rdf:about="http://purl.org/ppeo/MDO.owl#includesAtMostOne">
        <rdfs:subPropertyOf rdf:resource="http://purl.org/ppeo/MDO.owl#includes"/>
        <rdfs:domain rdf:resource="http://purl.org/ppeo/MDO.owl#object"/>
        <rdfs:range rdf:resource="http://purl.org/ppeo/MDO.owl#metadata_entity"/>
        <rdfs:label xml:lang="en">includes at most one</rdfs:label>
    </owl:ObjectProperty>
    


    <!-- http://purl.org/ppeo/MDO.owl#includesExactlyOne -->

    <owl:ObjectProperty rdf:about="http://purl.org/ppeo/MDO.owl#includesExactlyOne">
        <rdfs:subPropertyOf rdf:resource="http://purl.org/ppeo/MDO.owl#includes"/>
        <rdfs:domain rdf:resource="http://purl.org/ppeo/MDO.owl#object"/>
        <rdfs:range rdf:resource="http://purl.org/ppeo/MDO.owl#metadata_entity"/>
        <rdfs:label xml:lang="en">includes exactly one</rdfs:label>
    </owl:ObjectProperty>
    


    <!-- http://purl.org/ppeo/MDO.owl#includesMoreThanOne -->

    <owl:ObjectProperty rdf:about="http://purl.org/ppeo/MDO.owl#includesMoreThanOne">
        <rdfs:subPropertyOf rdf:resource="http://purl.org/ppeo/MDO.owl#includes"/>
        <rdfs:domain rdf:resource="http://purl.org/ppeo/MDO.owl#object"/>
        <rdfs:range rdf:resource="http://purl.org/ppeo/MDO.owl#metadata_entity"/>
        <rdfs:label xml:lang="en">includes more than one</rdfs:label>
    </owl:ObjectProperty>
    


    <!-- http://purl.org/ppeo/MDO.owl#references -->

    <owl:ObjectProperty rdf:about="http://purl.org/ppeo/MDO.owl#references">
        <rdfs:domain rdf:resource="http://purl.org/ppeo/MDO.owl#selection_field"/>
        <rdfs:range rdf:resource="http://purl.org/ppeo/MDO.owl#enumeration_field"/>
        <rdfs:comment xml:lang="en">Used to connect two fields, when a selection must be made from the object field (enumeration) for the subject field (selection field).</rdfs:comment>
        <rdfs:label xml:lang="en">references</rdfs:label>
    </owl:ObjectProperty>
    


    <!-- 
    ///////////////////////////////////////////////////////////////////////////////////////
    //
    // Data properties
    //
    ///////////////////////////////////////////////////////////////////////////////////////
     -->

    


    <!-- http://purl.org/ppeo/MDO.owl#hasDataType -->

    <owl:DatatypeProperty rdf:about="http://purl.org/ppeo/MDO.owl#hasDataType">
        <rdfs:domain rdf:resource="http://purl.org/ppeo/MDO.owl#field"/>
        <rdfs:range rdf:resource="http://www.w3.org/2000/01/rdf-schema#Literal"/>
        <rdfs:comment xml:lang="en">Indicates the type of data (e.g. string, number, date) that is expected in a Fixed datatype field. A pattern can also be defined using regular expressions (e.g. xsd:string[pattern &quot;[0-9]{5}(-[0-9]{4})?&quot;]).</rdfs:comment>
        <rdfs:label xml:lang="en">data type</rdfs:label>
    </owl:DatatypeProperty>
    


    <!-- http://purl.org/ppeo/MDO.owl#hasDefinition -->

    <owl:DatatypeProperty rdf:about="http://purl.org/ppeo/MDO.owl#hasDefinition">
        <rdf:type rdf:resource="http://www.w3.org/2002/07/owl#FunctionalProperty"/>
        <rdfs:domain rdf:resource="http://purl.org/ppeo/MDO.owl#metadata_entity"/>
        <rdfs:range rdf:resource="http://www.w3.org/2001/XMLSchema#string"/>
        <rdfs:comment xml:lang="en">Shows the definition for fields that the users have to fill in.</rdfs:comment>
        <rdfs:label xml:lang="en">definition</rdfs:label>
    </owl:DatatypeProperty>
    


    <!-- http://purl.org/ppeo/MDO.owl#hasDisplayName -->

    <owl:DatatypeProperty rdf:about="http://purl.org/ppeo/MDO.owl#hasDisplayName">
        <rdf:type rdf:resource="http://www.w3.org/2002/07/owl#FunctionalProperty"/>
        <rdfs:domain rdf:resource="http://purl.org/ppeo/MDO.owl#metadata_entity"/>
        <rdfs:range rdf:resource="http://www.w3.org/2001/XMLSchema#string"/>
        <rdfs:comment xml:lang="en">The name of the fields/section/object that will be shown on the interface.</rdfs:comment>
        <rdfs:label xml:lang="en">display name</rdfs:label>
    </owl:DatatypeProperty>
    


    <!-- http://purl.org/ppeo/MDO.owl#hasExample -->

    <owl:DatatypeProperty rdf:about="http://purl.org/ppeo/MDO.owl#hasExample">
        <rdfs:domain rdf:resource="http://purl.org/ppeo/MDO.owl#field"/>
        <rdfs:range rdf:resource="http://www.w3.org/2001/XMLSchema#string"/>
        <rdfs:comment xml:lang="en">An example value for a field.</rdfs:comment>
        <rdfs:label xml:lang="en">example</rdfs:label>
    </owl:DatatypeProperty>
    


    <!-- http://purl.org/ppeo/MDO.owl#hasOntologyRecommendation -->

    <owl:DatatypeProperty rdf:about="http://purl.org/ppeo/MDO.owl#hasOntologyRecommendation">
        <rdfs:domain rdf:resource="http://purl.org/ppeo/MDO.owl#field"/>
        <rdfs:range>
            <rdfs:Datatype>
                <owl:unionOf rdf:parseType="Collection">
                    <rdf:Description rdf:about="http://www.w3.org/2001/XMLSchema#anyURI"/>
                    <rdf:Description rdf:about="http://www.w3.org/2001/XMLSchema#string"/>
                </owl:unionOf>
            </rdfs:Datatype>
        </rdfs:range>
        <rdfs:comment xml:lang="en">Can be used to point to ontologies / controlled vocabularies for a field.</rdfs:comment>
        <rdfs:label xml:lang="en">ontology recommendation</rdfs:label>
    </owl:DatatypeProperty>
    


    <!-- http://purl.org/ppeo/MDO.owl#hasOrderFactor -->

    <owl:DatatypeProperty rdf:about="http://purl.org/ppeo/MDO.owl#hasOrderFactor">
        <rdfs:domain rdf:resource="http://purl.org/ppeo/MDO.owl#metadata_entity"/>
        <rdfs:range rdf:resource="http://www.w3.org/2001/XMLSchema#integer"/>
        <rdfs:comment xml:lang="en">A number used for ordering elements in the interface. Elements with a smaller number will appear first, then elements with a larger number. Order factor is irrelevant in between sections.</rdfs:comment>
        <rdfs:label xml:lang="en">order factor</rdfs:label>
    </owl:DatatypeProperty>
    


    <!-- http://purl.org/ppeo/MDO.owl#isTopSection -->

    <owl:DatatypeProperty rdf:about="http://purl.org/ppeo/MDO.owl#isTopSection">
        <rdf:type rdf:resource="http://www.w3.org/2002/07/owl#FunctionalProperty"/>
        <rdfs:domain rdf:resource="http://purl.org/ppeo/MDO.owl#section"/>
        <rdfs:range rdf:resource="http://www.w3.org/2001/XMLSchema#boolean"/>
        <rdfs:comment xml:lang="en">Marks a section that has no parent.</rdfs:comment>
        <rdfs:label xml:lang="en">top section</rdfs:label>
    </owl:DatatypeProperty>
    


    <!-- 
    ///////////////////////////////////////////////////////////////////////////////////////
    //
    // Classes
    //
    ///////////////////////////////////////////////////////////////////////////////////////
     -->

    


    <!-- http://purl.org/ppeo/MDO.owl#ID_field -->

    <owl:Class rdf:about="http://purl.org/ppeo/MDO.owl#ID_field">
        <rdfs:subClassOf rdf:resource="http://purl.org/ppeo/MDO.owl#field"/>
        <rdfs:comment xml:lang="en">A field holding the main identifier for the resource being described.</rdfs:comment>
        <rdfs:label xml:lang="en">ID field</rdfs:label>
    </owl:Class>
    


    <!-- http://purl.org/ppeo/MDO.owl#abstract_object -->

    <owl:Class rdf:about="http://purl.org/ppeo/MDO.owl#abstract_object">
        <rdfs:subClassOf rdf:resource="http://purl.org/ppeo/MDO.owl#object"/>
        <owl:disjointWith rdf:resource="http://purl.org/ppeo/MDO.owl#section"/>
        <rdfs:label xml:lang="en">abstract object</rdfs:label>
    </owl:Class>
    


    <!-- http://purl.org/ppeo/MDO.owl#controlled_vocabulary_field -->

    <owl:Class rdf:about="http://purl.org/ppeo/MDO.owl#controlled_vocabulary_field">
        <rdfs:subClassOf rdf:resource="http://purl.org/ppeo/MDO.owl#field"/>
        <rdfs:comment xml:lang="en">A field that is expected to take values from a recommended external ontology or controlled vocabulary, but also accepts free-text values if no suitable ontology concepts exist.</rdfs:comment>
        <rdfs:label xml:lang="en">controlled vocabulary field</rdfs:label>
    </owl:Class>
    


    <!-- http://purl.org/ppeo/MDO.owl#enumeration_field -->

    <owl:Class rdf:about="http://purl.org/ppeo/MDO.owl#enumeration_field">
        <rdfs:subClassOf rdf:resource="http://purl.org/ppeo/MDO.owl#field"/>
        <rdfs:comment xml:lang="en">A field that expects a list  of possible values. It can be paired with a selection field to allow the user to specify any number of those values elsewhere in the metadata structure.</rdfs:comment>
        <rdfs:label xml:lang="en">enumeration field</rdfs:label>
    </owl:Class>
    


    <!-- http://purl.org/ppeo/MDO.owl#field -->

    <owl:Class rdf:about="http://purl.org/ppeo/MDO.owl#field">
        <rdfs:subClassOf rdf:resource="http://purl.org/ppeo/MDO.owl#metadata_entity"/>
        <owl:disjointWith rdf:resource="http://purl.org/ppeo/MDO.owl#object"/>
        <rdfs:comment xml:lang="en">A metadata field (or attribute) for which the user is expected to enter a value.</rdfs:comment>
        <rdfs:label xml:lang="en">field</rdfs:label>
    </owl:Class>
    


    <!-- http://purl.org/ppeo/MDO.owl#fixed_datatype_field -->

    <owl:Class rdf:about="http://purl.org/ppeo/MDO.owl#fixed_datatype_field">
        <rdfs:subClassOf rdf:resource="http://purl.org/ppeo/MDO.owl#field"/>
        <rdfs:comment xml:lang="en">A field where a specified value type is expected  (e.g. number, date).</rdfs:comment>
        <rdfs:label xml:lang="en">fixed datatype field</rdfs:label>
    </owl:Class>
    


    <!-- http://purl.org/ppeo/MDO.owl#free_value_field -->

    <owl:Class rdf:about="http://purl.org/ppeo/MDO.owl#free_value_field">
        <rdfs:subClassOf rdf:resource="http://purl.org/ppeo/MDO.owl#field"/>
        <rdfs:comment xml:lang="en">A field where any value can be entered without type restrictions but with expected short length.</rdfs:comment>
        <rdfs:label xml:lang="en">free value field</rdfs:label>
    </owl:Class>
    


    <!-- http://purl.org/ppeo/MDO.owl#long_text_field -->

    <owl:Class rdf:about="http://purl.org/ppeo/MDO.owl#long_text_field">
        <rdfs:subClassOf rdf:resource="http://purl.org/ppeo/MDO.owl#field"/>
        <rdfs:comment xml:lang="en">A field where long free text can be entered, typically used for detailed descriptions.</rdfs:comment>
        <rdfs:label xml:lang="en">long text field</rdfs:label>
    </owl:Class>
    


    <!-- http://purl.org/ppeo/MDO.owl#metadata_entity -->

    <owl:Class rdf:about="http://purl.org/ppeo/MDO.owl#metadata_entity">
        <owl:equivalentClass>
            <owl:Class>
                <owl:unionOf rdf:parseType="Collection">
                    <rdf:Description rdf:about="http://purl.org/ppeo/MDO.owl#field"/>
                    <rdf:Description rdf:about="http://purl.org/ppeo/MDO.owl#object"/>
                </owl:unionOf>
            </owl:Class>
        </owl:equivalentClass>
        <rdfs:comment xml:lang="en">A metadata entity, which can be a field XOR an object (grouping fields)</rdfs:comment>
        <rdfs:label xml:lang="en">metadata entity</rdfs:label>
    </owl:Class>
    


    <!-- http://purl.org/ppeo/MDO.owl#object -->

    <owl:Class rdf:about="http://purl.org/ppeo/MDO.owl#object">
        <rdfs:subClassOf rdf:resource="http://purl.org/ppeo/MDO.owl#metadata_entity"/>
        <rdfs:comment xml:lang="en">An entity that requires (typically multiple) fields to describe. It may also contain other sub-objects.</rdfs:comment>
        <rdfs:label xml:lang="en">object</rdfs:label>
    </owl:Class>
    


    <!-- http://purl.org/ppeo/MDO.owl#restriction_field -->

    <owl:Class rdf:about="http://purl.org/ppeo/MDO.owl#restriction_field">
        <rdfs:subClassOf rdf:resource="http://purl.org/ppeo/MDO.owl#selection_field"/>
        <rdfs:comment xml:lang="en">A field that can only take a single value from a specified enumeration field.</rdfs:comment>
        <rdfs:label xml:lang="en">restriction field</rdfs:label>
    </owl:Class>
    


    <!-- http://purl.org/ppeo/MDO.owl#section -->

    <owl:Class rdf:about="http://purl.org/ppeo/MDO.owl#section">
        <rdfs:subClassOf rdf:resource="http://purl.org/ppeo/MDO.owl#object"/>
        <rdfs:comment xml:lang="en">An object that should be visualized on its own, typically because it contains numerous fields or sub-objects and/or because it represents a conceptually independent portion of a metadata scheme.</rdfs:comment>
        <rdfs:label xml:lang="en">section</rdfs:label>
    </owl:Class>
    


    <!-- http://purl.org/ppeo/MDO.owl#selection_field -->

    <owl:Class rdf:about="http://purl.org/ppeo/MDO.owl#selection_field">
        <rdfs:subClassOf rdf:resource="http://purl.org/ppeo/MDO.owl#field"/>
        <rdfs:comment xml:lang="en">A field that can only take values from among those listed in a specified  enumeration field.</rdfs:comment>
        <rdfs:label xml:lang="en">selection field</rdfs:label>
    </owl:Class>
</rdf:RDF>



<!-- Generated by the OWL API (version 4.5.9.2019-02-01T07:24:44Z) https://github.com/owlcs/owlapi -->

